<?xml version="1.0"?>


<!DOCTYPE rdf:RDF [
    <!ENTITY owl "http://www.w3.org/2002/07/owl#" >
    <!ENTITY obo "http://purl.obolibrary.org/obo/" >
    <!ENTITY dc "http://purl.org/dc/elements/1.1/" >
    <!ENTITY xsd "http://www.w3.org/2001/XMLSchema#" >
    <!ENTITY rdfs "http://www.w3.org/2000/01/rdf-schema#" >
    <!ENTITY rdf "http://www.w3.org/1999/02/22-rdf-syntax-ns#" >
]>


<rdf:RDF xmlns="http://josh.hanna.io/ontologies/twitter.owl#"
     xml:base="http://josh.hanna.io/ontologies/twitter.owl"
     xmlns:dc="http://purl.org/dc/elements/1.1/"
     xmlns:obo="http://purl.obolibrary.org/obo/"
     xmlns:rdfs="http://www.w3.org/2000/01/rdf-schema#"
     xmlns:owl="http://www.w3.org/2002/07/owl#"
     xmlns:xsd="http://www.w3.org/2001/XMLSchema#"
     xmlns:rdf="http://www.w3.org/1999/02/22-rdf-syntax-ns#">
    <owl:Ontology rdf:about="http://josh.hanna.io/ontologies/twitter.owl">
        <dc:creator>Josh Hanna</dc:creator>
        <dc:description>An ontology of Twitter data items.</dc:description>
        <owl:imports rdf:resource="&obo;iao.owl"/>
    </owl:Ontology>
    


    <!-- 
    ///////////////////////////////////////////////////////////////////////////////////////
    //
    // Data properties
    //
    ///////////////////////////////////////////////////////////////////////////////////////
     -->

    


    <!-- http://josh.hanna.io/ontologies/twitter.owl/TWITTER_00000031 -->

    <owl:DatatypeProperty rdf:about="http://josh.hanna.io/ontologies/twitter.owl/TWITTER_00000031">
        <rdfs:label xml:lang="en">has asserted value</rdfs:label>
        <obo:IAO_0000115>A relation that holds between an entity and a value that has been asserted to be true.</obo:IAO_0000115>
        <rdfs:domain rdf:resource="&obo;IAO_0000027"/>
        <rdfs:range>
            <rdfs:Datatype>
                <owl:unionOf rdf:parseType="Collection">
                    <rdf:Description rdf:about="&xsd;boolean"/>
                    <rdf:Description rdf:about="&xsd;dateTime"/>
                    <rdf:Description rdf:about="&xsd;decimal"/>
                    <rdf:Description rdf:about="&xsd;double"/>
                    <rdf:Description rdf:about="&xsd;float"/>
                    <rdf:Description rdf:about="&xsd;int"/>
                    <rdf:Description rdf:about="&xsd;integer"/>
                    <rdf:Description rdf:about="&xsd;string"/>
                </owl:unionOf>
            </rdfs:Datatype>
        </rdfs:range>
    </owl:DatatypeProperty>
    


    <!-- 
    ///////////////////////////////////////////////////////////////////////////////////////
    //
    // Classes
    //
    ///////////////////////////////////////////////////////////////////////////////////////
     -->

    


    <!-- http://josh.hanna.io/ontologies/twitter.owl/TWITTER_00000001 -->

    <owl:Class rdf:about="http://josh.hanna.io/ontologies/twitter.owl/TWITTER_00000001">
        <rdfs:label xml:lang="en">tweet data item</rdfs:label>
        <rdfs:subClassOf rdf:resource="&obo;IAO_0000027"/>
        <obo:IAO_0000115>A data item containing other data items, including the message that was shared, the time the message was created, and various data items that are about the human or computer system that generated the message.</obo:IAO_0000115>
    </owl:Class>
    


    <!-- http://josh.hanna.io/ontologies/twitter.owl/TWITTER_00000002 -->

    <owl:Class rdf:about="http://josh.hanna.io/ontologies/twitter.owl/TWITTER_00000002">
        <rdfs:label xml:lang="en">tweet message</rdfs:label>
        <rdfs:subClassOf rdf:resource="http://josh.hanna.io/ontologies/twitter.owl/TWITTER_00000003"/>
        <obo:IAO_0000115>The textual message generated by the person or computer system that was shared via a tweet data item.</obo:IAO_0000115>
    </owl:Class>
    


    <!-- http://josh.hanna.io/ontologies/twitter.owl/TWITTER_00000003 -->

    <owl:Class rdf:about="http://josh.hanna.io/ontologies/twitter.owl/TWITTER_00000003">
        <rdfs:label xml:lang="en">tweet data item part</rdfs:label>
        <owl:equivalentClass>
            <owl:Restriction>
                <owl:onProperty rdf:resource="http://www.obofoundry.org/ro/ro.owl#part_of"/>
                <owl:someValuesFrom rdf:resource="http://josh.hanna.io/ontologies/twitter.owl/TWITTER_00000001"/>
            </owl:Restriction>
        </owl:equivalentClass>
        <rdfs:subClassOf rdf:resource="&obo;IAO_0000027"/>
    </owl:Class>
    


    <!-- http://josh.hanna.io/ontologies/twitter.owl/TWITTER_00000004 -->

    <owl:Class rdf:about="http://josh.hanna.io/ontologies/twitter.owl/TWITTER_00000004">
        <rdfs:label xml:lang="en">data set containing contributors ids</rdfs:label>
        <rdfs:subClassOf rdf:resource="http://josh.hanna.io/ontologies/twitter.owl/TWITTER_00000003"/>
        <rdfs:comment>Twitter Guidance: An collection of brief user objects (usually only one) indicating users who contributed to the authorship of the tweet, on behalf of the official tweet author.</rdfs:comment>
        <obo:IAO_0000115>A data set containing a list of identifiers that uniquely identify Twitter user accounts that contributed in some way to a tweet data item.</obo:IAO_0000115>
    </owl:Class>
    


    <!-- http://josh.hanna.io/ontologies/twitter.owl/TWITTER_00000005 -->

    <owl:Class rdf:about="http://josh.hanna.io/ontologies/twitter.owl/TWITTER_00000005">
        <rdfs:label xml:lang="en">longitude of the location tweet was generated</rdfs:label>
        <rdfs:subClassOf rdf:resource="http://josh.hanna.io/ontologies/twitter.owl/TWITTER_00000003"/>
        <obo:IAO_0000115>A measurement of the longitude by some geopositioning device of the location where the tweet data item was generated.</obo:IAO_0000115>
    </owl:Class>
    


    <!-- http://josh.hanna.io/ontologies/twitter.owl/TWITTER_00000006 -->

    <owl:Class rdf:about="http://josh.hanna.io/ontologies/twitter.owl/TWITTER_00000006">
        <rdfs:label xml:lang="en">latitude of the location tweet was generated</rdfs:label>
        <rdfs:subClassOf rdf:resource="http://josh.hanna.io/ontologies/twitter.owl/TWITTER_00000003"/>
        <obo:IAO_0000115>A measurement of the latitude by some geopositioning device of the location where the tweet data item was generated.</obo:IAO_0000115>
    </owl:Class>
    


    <!-- http://josh.hanna.io/ontologies/twitter.owl/TWITTER_00000007 -->

    <owl:Class rdf:about="http://josh.hanna.io/ontologies/twitter.owl/TWITTER_00000007">
        <rdfs:label xml:lang="en">created timestamp</rdfs:label>
        <owl:equivalentClass>
            <owl:Restriction>
                <owl:onProperty rdf:resource="&obo;IAO_0000136"/>
                <owl:someValuesFrom>
                    <owl:Class>
                        <owl:intersectionOf rdf:parseType="Collection">
                            <rdf:Description rdf:about="&obo;IAO_0000416"/>
                            <owl:Restriction>
                                <owl:onProperty rdf:resource="&obo;IAO_0000136"/>
                                <owl:someValuesFrom rdf:resource="http://josh.hanna.io/ontologies/twitter.owl/TWITTER_00000001"/>
                            </owl:Restriction>
                        </owl:intersectionOf>
                    </owl:Class>
                </owl:someValuesFrom>
            </owl:Restriction>
        </owl:equivalentClass>
        <rdfs:subClassOf rdf:resource="http://josh.hanna.io/ontologies/twitter.owl/TWITTER_00000003"/>
        <obo:IAO_0000115>A timestamp which denotes the precise time during which a tweet data item was created.</obo:IAO_0000115>
    </owl:Class>
    


    <!-- http://josh.hanna.io/ontologies/twitter.owl/TWITTER_00000008 -->

    <owl:Class rdf:about="http://josh.hanna.io/ontologies/twitter.owl/TWITTER_00000008">
        <rdfs:label xml:lang="en">data set containing hashtags</rdfs:label>
        <rdfs:subClassOf rdf:resource="http://josh.hanna.io/ontologies/twitter.owl/TWITTER_00000003"/>
        <rdfs:subClassOf rdf:resource="&obo;IAO_0000100"/>
        <obo:IAO_0000115>A data set containing a list of strings which a users uses to denote the topic(s) of a tweet message.</obo:IAO_0000115>
    </owl:Class>
    


    <!-- http://josh.hanna.io/ontologies/twitter.owl/TWITTER_00000009 -->

    <owl:Class rdf:about="http://josh.hanna.io/ontologies/twitter.owl/TWITTER_00000009">
        <rdfs:label xml:lang="en">data set containing tweet-relevant urls</rdfs:label>
        <rdfs:subClassOf rdf:resource="http://josh.hanna.io/ontologies/twitter.owl/TWITTER_00000003"/>
        <rdfs:subClassOf rdf:resource="&obo;IAO_0000100"/>
        <obo:IAO_0000115>A data set containing a list of URLs that are relevant to the tweet data item by some metric.</obo:IAO_0000115>
    </owl:Class>
    


    <!-- http://josh.hanna.io/ontologies/twitter.owl/TWITTER_00000010 -->

    <owl:Class rdf:about="http://josh.hanna.io/ontologies/twitter.owl/TWITTER_00000010">
        <rdfs:label xml:lang="en">data set containing mentioned user ids</rdfs:label>
        <rdfs:subClassOf rdf:resource="http://josh.hanna.io/ontologies/twitter.owl/TWITTER_00000003"/>
        <rdfs:subClassOf rdf:resource="&obo;IAO_0000100"/>
        <obo:IAO_0000115>A data set containing a list of identifiers which denote a user account which has been mentioned directly in the tweet message.</obo:IAO_0000115>
    </owl:Class>
    


    <!-- http://josh.hanna.io/ontologies/twitter.owl/TWITTER_00000011 -->

    <owl:Class rdf:about="http://josh.hanna.io/ontologies/twitter.owl/TWITTER_00000011">
        <rdfs:label xml:lang="en">retweet data item</rdfs:label>
        <rdfs:subClassOf rdf:resource="http://josh.hanna.io/ontologies/twitter.owl/TWITTER_00000003"/>
    </owl:Class>
    


    <!-- http://josh.hanna.io/ontologies/twitter.owl/TWITTER_00000012 -->

    <owl:Class rdf:about="http://josh.hanna.io/ontologies/twitter.owl/TWITTER_00000012">
        <rdfs:label xml:lang="en">count of users who favorited</rdfs:label>
        <owl:equivalentClass>
            <owl:Restriction>
                <owl:onProperty rdf:resource="&obo;IAO_0000136"/>
                <owl:someValuesFrom>
                    <owl:Class>
                        <owl:intersectionOf rdf:parseType="Collection">
                            <rdf:Description rdf:about="&obo;IAO_0000109"/>
                            <owl:Restriction>
                                <owl:onProperty rdf:resource="&obo;IAO_0000136"/>
                                <owl:someValuesFrom rdf:resource="http://josh.hanna.io/ontologies/twitter.owl/TWITTER_00000034"/>
                            </owl:Restriction>
                        </owl:intersectionOf>
                    </owl:Class>
                </owl:someValuesFrom>
            </owl:Restriction>
        </owl:equivalentClass>
        <rdfs:subClassOf rdf:resource="http://josh.hanna.io/ontologies/twitter.owl/TWITTER_00000003"/>
        <rdfs:comment>Twitter Guidance: Indicates approximately how many times this Tweet has been &quot;favorited&quot; by Twitter users.</rdfs:comment>
    </owl:Class>
    


    <!-- http://josh.hanna.io/ontologies/twitter.owl/TWITTER_00000013 -->

    <owl:Class rdf:about="http://josh.hanna.io/ontologies/twitter.owl/TWITTER_00000013">
        <rdfs:label xml:lang="en">favorited flag</rdfs:label>
        <owl:equivalentClass>
            <owl:Restriction>
                <owl:onProperty rdf:resource="&obo;IAO_0000136"/>
                <owl:someValuesFrom>
                    <owl:Class>
                        <owl:intersectionOf rdf:parseType="Collection">
                            <rdf:Description rdf:about="http://josh.hanna.io/ontologies/twitter.owl/TWITTER_00000001"/>
                            <owl:Restriction>
                                <owl:onProperty rdf:resource="http://www.obofoundry.org/ro/ro.owl#participates_in"/>
                                <owl:someValuesFrom rdf:resource="http://josh.hanna.io/ontologies/twitter.owl/TWITTER_00000034"/>
                            </owl:Restriction>
                        </owl:intersectionOf>
                    </owl:Class>
                </owl:someValuesFrom>
            </owl:Restriction>
        </owl:equivalentClass>
        <rdfs:subClassOf rdf:resource="http://josh.hanna.io/ontologies/twitter.owl/TWITTER_00000003"/>
        <obo:IAO_0000115>A flag which denotes whether or not a user has particpated in the favoriting process at least one more than they have participated in a reverse process.</obo:IAO_0000115>
    </owl:Class>
    


    <!-- http://josh.hanna.io/ontologies/twitter.owl/TWITTER_00000014 -->

    <owl:Class rdf:about="http://josh.hanna.io/ontologies/twitter.owl/TWITTER_00000014">
        <rdfs:label xml:lang="en">filter level</rdfs:label>
        <rdfs:subClassOf rdf:resource="http://josh.hanna.io/ontologies/twitter.owl/TWITTER_00000003"/>
        <rdfs:comment>Twitter Guidance: Indicates the maximum value of the filter_level parameter which may be used and still stream this Tweet. So a value of medium will be streamed on none, low, and medium streams.</rdfs:comment>
    </owl:Class>
    


    <!-- http://josh.hanna.io/ontologies/twitter.owl/TWITTER_00000015 -->

    <owl:Class rdf:about="http://josh.hanna.io/ontologies/twitter.owl/TWITTER_00000015">
        <rdfs:label xml:lang="en">tweet id</rdfs:label>
        <rdfs:subClassOf rdf:resource="http://josh.hanna.io/ontologies/twitter.owl/TWITTER_00000003"/>
        <rdfs:subClassOf rdf:resource="&obo;IAO_0000578"/>
        <obo:IAO_0000115>A centrally registered identifier that denotes a tweet data item.</obo:IAO_0000115>
        <rdfs:comment>Twitter Guidance: The integer representation of the unique identifier for this Tweet. This number is greater than 53 bits and some programming languages may have difficulty/silent defects in interpreting it. Using a signed 64 bit integer for storing this identifier is safe. Use id_str for fetching the identifier to stay on the safe side.</rdfs:comment>
    </owl:Class>
    


    <!-- http://josh.hanna.io/ontologies/twitter.owl/TWITTER_00000016 -->

    <owl:Class rdf:about="http://josh.hanna.io/ontologies/twitter.owl/TWITTER_00000016">
        <rdfs:label xml:lang="en">user screen name responded to</rdfs:label>
        <rdfs:subClassOf rdf:resource="http://josh.hanna.io/ontologies/twitter.owl/TWITTER_00000003"/>
        <obo:IAO_0000115>An identifier that, at some point in time, uniquely identifies a Twitter user account.</obo:IAO_0000115>
        <rdfs:comment>Twitter Guidance: If the represented Tweet is a reply, this field will contain the screen name of the original Tweet&apos;s author.</rdfs:comment>
    </owl:Class>
    


    <!-- http://josh.hanna.io/ontologies/twitter.owl/TWITTER_00000017 -->

    <owl:Class rdf:about="http://josh.hanna.io/ontologies/twitter.owl/TWITTER_00000017">
        <rdfs:label xml:lang="en">tweet id responded to</rdfs:label>
        <rdfs:subClassOf rdf:resource="http://josh.hanna.io/ontologies/twitter.owl/TWITTER_00000003"/>
        <obo:IAO_0000115>A identifier that denotes a tweet data item that the associated tweet data item was created in response to.</obo:IAO_0000115>
        <rdfs:comment>Twitter Guidance: If the represented Tweet is a reply, this field will contain the integer representation of the original Tweet&apos;s ID.</rdfs:comment>
    </owl:Class>
    


    <!-- http://josh.hanna.io/ontologies/twitter.owl/TWITTER_00000018 -->

    <owl:Class rdf:about="http://josh.hanna.io/ontologies/twitter.owl/TWITTER_00000018">
        <rdfs:label xml:lang="en">user id responded to</rdfs:label>
        <rdfs:subClassOf rdf:resource="http://josh.hanna.io/ontologies/twitter.owl/TWITTER_00000003"/>
        <obo:IAO_0000115>An identifier that denotes a user which is the intended recepient of the associated tweet message.</obo:IAO_0000115>
    </owl:Class>
    


    <!-- http://josh.hanna.io/ontologies/twitter.owl/TWITTER_00000019 -->

    <owl:Class rdf:about="http://josh.hanna.io/ontologies/twitter.owl/TWITTER_00000019">
        <rdfs:label xml:lang="en">tweet language</rdfs:label>
        <rdfs:subClassOf rdf:resource="http://josh.hanna.io/ontologies/twitter.owl/TWITTER_00000003"/>
        <rdfs:comment>Twitter Guidance: When present, indicates a BCP 47 language identifier corresponding to the machine-detected language of the Tweet text, or &quot;und&quot; if no language could be detected.</rdfs:comment>
        <obo:IAO_0000115>A data item that is about the language that a tweet message is written in.</obo:IAO_0000115>
    </owl:Class>
    


    <!-- http://josh.hanna.io/ontologies/twitter.owl/TWITTER_00000020 -->

    <owl:Class rdf:about="http://josh.hanna.io/ontologies/twitter.owl/TWITTER_00000020">
        <rdfs:label xml:lang="en">data set containing associated geographical regions</rdfs:label>
        <rdfs:subClassOf rdf:resource="http://josh.hanna.io/ontologies/twitter.owl/TWITTER_00000003"/>
        <obo:IAO_0000115>A data set containing a list of geographical regions which are relevant by some metric to a tweet data item.</obo:IAO_0000115>
    </owl:Class>
    


    <!-- http://josh.hanna.io/ontologies/twitter.owl/TWITTER_00000021 -->

    <owl:Class rdf:about="http://josh.hanna.io/ontologies/twitter.owl/TWITTER_00000021">
        <rdfs:label xml:lang="en">sensitive content flag</rdfs:label>
        <rdfs:subClassOf rdf:resource="http://josh.hanna.io/ontologies/twitter.owl/TWITTER_00000003"/>
        <obo:IAO_0000115>A boolean value that denotes whether or not the associated tweet message contains a URL which links content deemed sensitive by some metric.</obo:IAO_0000115>
        <rdfs:comment>Twitter Guidance: This field only surfaces when a tweet contains a link. The meaning of the field doesn&apos;t pertain to the tweet content itself, but instead it is an indicator that the URL contained in the tweet may contain content or media identified as sensitive content.</rdfs:comment>
    </owl:Class>
    


    <!-- http://josh.hanna.io/ontologies/twitter.owl/TWITTER_00000022 -->

    <owl:Class rdf:about="http://josh.hanna.io/ontologies/twitter.owl/TWITTER_00000022">
        <rdfs:label xml:lang="en">count of retweets</rdfs:label>
        <owl:equivalentClass>
            <owl:Restriction>
                <owl:onProperty rdf:resource="&obo;IAO_0000136"/>
                <owl:someValuesFrom>
                    <owl:Class>
                        <owl:intersectionOf rdf:parseType="Collection">
                            <rdf:Description rdf:about="&obo;IAO_0000109"/>
                            <owl:Restriction>
                                <owl:onProperty rdf:resource="&obo;IAO_0000136"/>
                                <owl:someValuesFrom rdf:resource="http://josh.hanna.io/ontologies/twitter.owl/TWITTER_00000033"/>
                            </owl:Restriction>
                        </owl:intersectionOf>
                    </owl:Class>
                </owl:someValuesFrom>
            </owl:Restriction>
        </owl:equivalentClass>
        <rdfs:subClassOf rdf:resource="http://josh.hanna.io/ontologies/twitter.owl/TWITTER_00000003"/>
        <rdfs:comment>TODO: I need to grab an actual count measurement class.  I believe apollo has one.</rdfs:comment>
        <rdfs:comment>Twitter Guidance: Number of times this Tweet has been retweeted. This field is no longer capped at 99 and will not turn into a String for &quot;100+&quot;.</rdfs:comment>
        <obo:IAO_0000115>A count of the number of times the associated tweet message has been retweeted.</obo:IAO_0000115>
    </owl:Class>
    


    <!-- http://josh.hanna.io/ontologies/twitter.owl/TWITTER_00000023 -->

    <owl:Class rdf:about="http://josh.hanna.io/ontologies/twitter.owl/TWITTER_00000023">
        <rdfs:label xml:lang="en">retweeted flag</rdfs:label>
        <rdfs:subClassOf rdf:resource="http://josh.hanna.io/ontologies/twitter.owl/TWITTER_00000003"/>
        <obo:IAO_0000115>A data item which denotes whether or not the associated tweet data item is original or participating in the retweeting process.</obo:IAO_0000115>
    </owl:Class>
    


    <!-- http://josh.hanna.io/ontologies/twitter.owl/TWITTER_00000024 -->

    <owl:Class rdf:about="http://josh.hanna.io/ontologies/twitter.owl/TWITTER_00000024">
        <rdfs:label xml:lang="en">retweeted tweet</rdfs:label>
        <rdfs:subClassOf rdf:resource="http://josh.hanna.io/ontologies/twitter.owl/TWITTER_00000003"/>
        <obo:IAO_0000115>A tweet data item that is participating in the retweeting process by being retweeted.</obo:IAO_0000115>
        <rdfs:comment>Twitter Guidance: Users can amplify the broadcast of tweets authored by other users by retweeting. Retweets can be distinguished from typical Tweets by the existence of a retweeted_status attribute. This attribute contains a representation of the original Tweet that was retweeted. Note that retweets of retweets do not show representations of the intermediary retweet, but only the original tweet. (Users can also unretweet a retweet they created by deleting their retweet.)</rdfs:comment>
    </owl:Class>
    


    <!-- http://josh.hanna.io/ontologies/twitter.owl/TWITTER_00000025 -->

    <owl:Class rdf:about="http://josh.hanna.io/ontologies/twitter.owl/TWITTER_00000025">
        <rdfs:label xml:lang="en">data item about the application used to generate tweet</rdfs:label>
        <owl:equivalentClass>
            <owl:Class>
                <owl:intersectionOf rdf:parseType="Collection">
                    <owl:Restriction>
                        <owl:onProperty rdf:resource="&obo;IAO_0000136"/>
                        <owl:someValuesFrom rdf:resource="http://josh.hanna.io/ontologies/twitter.owl/TWITTER_00000001"/>
                    </owl:Restriction>
                    <owl:Restriction>
                        <owl:onProperty rdf:resource="&obo;IAO_0000136"/>
                        <owl:someValuesFrom>
                            <owl:Class>
                                <owl:intersectionOf rdf:parseType="Collection">
                                    <rdf:Description rdf:about="&obo;IAO_0000594"/>
                                    <owl:Restriction>
                                        <owl:onProperty rdf:resource="http://www.obofoundry.org/ro/ro.owl#participates_in"/>
                                        <owl:someValuesFrom rdf:resource="http://josh.hanna.io/ontologies/twitter.owl/TWITTER_00000035"/>
                                    </owl:Restriction>
                                </owl:intersectionOf>
                            </owl:Class>
                        </owl:someValuesFrom>
                    </owl:Restriction>
                </owl:intersectionOf>
            </owl:Class>
        </owl:equivalentClass>
        <rdfs:subClassOf rdf:resource="http://josh.hanna.io/ontologies/twitter.owl/TWITTER_00000003"/>
        <rdfs:comment>Twitter Guidance: Utility used to post the Tweet, as an HTML-formatted string. Tweets from the Twitter website have a source value of web.</rdfs:comment>
        <obo:IAO_0000115>A possibly non-unique identifier that denotes the software application used to generate a tweet data item.</obo:IAO_0000115>
    </owl:Class>
    


    <!-- http://josh.hanna.io/ontologies/twitter.owl/TWITTER_00000026 -->

    <owl:Class rdf:about="http://josh.hanna.io/ontologies/twitter.owl/TWITTER_00000026">
        <rdfs:label xml:lang="en">truncated flag</rdfs:label>
        <rdfs:subClassOf rdf:resource="http://josh.hanna.io/ontologies/twitter.owl/TWITTER_00000003"/>
    </owl:Class>
    


    <!-- http://josh.hanna.io/ontologies/twitter.owl/TWITTER_00000027 -->

    <owl:Class rdf:about="http://josh.hanna.io/ontologies/twitter.owl/TWITTER_00000027">
        <rdfs:label xml:lang="en">tweet user</rdfs:label>
        <owl:equivalentClass>
            <owl:Class>
                <owl:intersectionOf rdf:parseType="Collection">
                    <rdf:Description rdf:about="http://josh.hanna.io/ontologies/twitter.owl/TWITTER_00000039"/>
                    <owl:Restriction>
                        <owl:onProperty rdf:resource="http://www.obofoundry.org/ro/ro.owl#part_of"/>
                        <owl:someValuesFrom rdf:resource="http://josh.hanna.io/ontologies/twitter.owl/TWITTER_00000001"/>
                    </owl:Restriction>
                </owl:intersectionOf>
            </owl:Class>
        </owl:equivalentClass>
        <rdfs:subClassOf rdf:resource="http://josh.hanna.io/ontologies/twitter.owl/TWITTER_00000003"/>
        <rdfs:comment>Twitter Guidance: The user who posted this Tweet. Perspectival attributes embedded within this object are unreliable.</rdfs:comment>
        <obo:IAO_0000115>A data item about the user account which generated the associated tweet data item.</obo:IAO_0000115>
    </owl:Class>
    


    <!-- http://josh.hanna.io/ontologies/twitter.owl/TWITTER_00000028 -->

    <owl:Class rdf:about="http://josh.hanna.io/ontologies/twitter.owl/TWITTER_00000028">
        <rdfs:label xml:lang="en">copyrighted flag</rdfs:label>
        <owl:equivalentClass>
            <owl:Restriction>
                <owl:onProperty rdf:resource="&obo;IAO_0000136"/>
                <owl:someValuesFrom rdf:resource="http://josh.hanna.io/ontologies/twitter.owl/TWITTER_00000032"/>
            </owl:Restriction>
        </owl:equivalentClass>
        <rdfs:subClassOf rdf:resource="http://josh.hanna.io/ontologies/twitter.owl/TWITTER_00000003"/>
        <obo:IAO_0000115>A boolean value that documents whether or not the tweet message is copyrighted.</obo:IAO_0000115>
        <rdfs:comment>TODO: Find the relationship that would hold between a copyright and a copyrighted entity (e.g., a creative work like a novel or software).</rdfs:comment>
    </owl:Class>
    


    <!-- http://josh.hanna.io/ontologies/twitter.owl/TWITTER_00000029 -->

    <owl:Class rdf:about="http://josh.hanna.io/ontologies/twitter.owl/TWITTER_00000029">
        <rdfs:label xml:lang="en">data set containing countries where tweet is disallowed</rdfs:label>
        <rdfs:subClassOf rdf:resource="http://josh.hanna.io/ontologies/twitter.owl/TWITTER_00000003"/>
        <rdfs:subClassOf rdf:resource="&obo;IAO_0000100"/>
        <obo:IAO_0000115>A data set containing geopolitical entities where a tweet data item is not allowed.</obo:IAO_0000115>
    </owl:Class>
    


    <!-- http://josh.hanna.io/ontologies/twitter.owl/TWITTER_00000032 -->

    <owl:Class rdf:about="http://josh.hanna.io/ontologies/twitter.owl/TWITTER_00000032">
        <rdfs:label xml:lang="en">copyright</rdfs:label>
        <rdfs:subClassOf rdf:resource="http://www.ifomis.org/bfo/1.1/snap#RealizableEntity"/>
        <obo:IAO_0000115>A realizable entity that adheres in some information content entity which confers certain legal rights to some entity.</obo:IAO_0000115>
    </owl:Class>
    


    <!-- http://josh.hanna.io/ontologies/twitter.owl/TWITTER_00000033 -->

    <owl:Class rdf:about="http://josh.hanna.io/ontologies/twitter.owl/TWITTER_00000033">
        <rdfs:label xml:lang="en">retweeting process</rdfs:label>
        <rdfs:subClassOf rdf:resource="http://www.ifomis.org/bfo/1.1/span#Process"/>
        <obo:IAO_0000115>A process by which a Twitter user shares the tweet message originally generated by a second user.</obo:IAO_0000115>
    </owl:Class>
    


    <!-- http://josh.hanna.io/ontologies/twitter.owl/TWITTER_00000034 -->

    <owl:Class rdf:about="http://josh.hanna.io/ontologies/twitter.owl/TWITTER_00000034">
        <rdfs:label xml:lang="en">favoriting process</rdfs:label>
        <rdfs:subClassOf rdf:resource="http://www.ifomis.org/bfo/1.1/span#Process"/>
        <obo:IAO_0000115>A process by which a Twitter user marks a specific tweet as a favorite.</obo:IAO_0000115>
    </owl:Class>
    


    <!-- http://josh.hanna.io/ontologies/twitter.owl/TWITTER_00000035 -->

    <owl:Class rdf:about="http://josh.hanna.io/ontologies/twitter.owl/TWITTER_00000035">
        <rdfs:label xml:lang="en">tweet generation process</rdfs:label>
        <rdfs:subClassOf rdf:resource="http://www.ifomis.org/bfo/1.1/span#Process"/>
    </owl:Class>
    


    <!-- http://josh.hanna.io/ontologies/twitter.owl/TWITTER_00000036 -->

    <owl:Class rdf:about="http://josh.hanna.io/ontologies/twitter.owl/TWITTER_00000036">
        <rdfs:label xml:lang="en">coordinates</rdfs:label>
        <owl:equivalentClass>
            <owl:Class>
                <owl:intersectionOf rdf:parseType="Collection">
                    <owl:Restriction>
                        <owl:onProperty rdf:resource="http://www.obofoundry.org/ro/ro.owl#has_part"/>
                        <owl:someValuesFrom rdf:resource="http://josh.hanna.io/ontologies/twitter.owl/TWITTER_00000005"/>
                    </owl:Restriction>
                    <owl:Restriction>
                        <owl:onProperty rdf:resource="http://www.obofoundry.org/ro/ro.owl#has_part"/>
                        <owl:someValuesFrom rdf:resource="http://josh.hanna.io/ontologies/twitter.owl/TWITTER_00000006"/>
                    </owl:Restriction>
                </owl:intersectionOf>
            </owl:Class>
        </owl:equivalentClass>
        <rdfs:subClassOf rdf:resource="http://josh.hanna.io/ontologies/twitter.owl/TWITTER_00000003"/>
        <obo:IAO_0000115>Represents the geographic location of this Tweet as reported by the user or client application.  Has two primary parts: a lattitude and a longitude</obo:IAO_0000115>
    </owl:Class>
    


    <!-- http://josh.hanna.io/ontologies/twitter.owl/TWITTER_00000039 -->

    <owl:Class rdf:about="http://josh.hanna.io/ontologies/twitter.owl/TWITTER_00000039">
        <rdfs:label xml:lang="en">twitter user data item</rdfs:label>
        <rdfs:subClassOf rdf:resource="&obo;IAO_0000027"/>
    </owl:Class>
    


    <!-- http://josh.hanna.io/ontologies/twitter.owl/TWITTER_00000040 -->

    <owl:Class rdf:about="http://josh.hanna.io/ontologies/twitter.owl/TWITTER_00000040">
        <rdfs:label xml:lang="en">twitter user data item part</rdfs:label>
        <rdfs:subClassOf rdf:resource="&obo;IAO_0000027"/>
    </owl:Class>
    


    <!-- http://josh.hanna.io/ontologies/twitter.owl/TWITTER_00000041 -->

    <owl:Class rdf:about="http://josh.hanna.io/ontologies/twitter.owl/TWITTER_00000041">
        <rdfs:label xml:lang="en">twitter user screen name</rdfs:label>
        <rdfs:subClassOf rdf:resource="http://josh.hanna.io/ontologies/twitter.owl/TWITTER_00000040"/>
        <rdfs:subClassOf rdf:resource="&obo;IAO_0000578"/>
    </owl:Class>
    


    <!-- http://josh.hanna.io/ontologies/twitter.owl/TWITTER_00000042 -->

    <owl:Class rdf:about="http://josh.hanna.io/ontologies/twitter.owl/TWITTER_00000042">
        <rdfs:label xml:lang="en">twitter user id</rdfs:label>
        <rdfs:subClassOf rdf:resource="http://josh.hanna.io/ontologies/twitter.owl/TWITTER_00000040"/>
        <rdfs:subClassOf rdf:resource="&obo;IAO_0000578"/>
    </owl:Class>
</rdf:RDF>



<!-- Generated by the OWL API (version 3.4.2) http://owlapi.sourceforge.net -->


